Starting to move TracedProgram building into inferred instance

HMem/Trace/Cost.lean
@@ -1,121 +1,150 @@
 import HMem.Trace.TracedProgram
 import HMem.Trace.Sound
 
-theorem Option.Forall_false: {o: Option α} → Option.Forall P o → (∀ a, ¬ P a ) → o = none
-| some _, hP, h => (h _ hP).recOn
-| none, _, _ => rfl
-
-def Option.Exists_exists: {o: Option α} → Option.Exists P o → (∃ a, o = some a ∧ P a)
-| some _, h => ⟨_, rfl, h⟩
-| none, h => absurd h not_false
-
 theorem Option.bind_of_none (h: o = none): Option.bind o f = none := h ▸ rfl
 
 namespace HMem.Trace
-variable {α: Type _} [Complexity.Encoding α Memory] {β: Type _} [Complexity.Encoding β Memory] {f: α → β} {tp: TracedProgram f}
+variable {α: Type _} [Complexity.Encoding α Memory] {β: Type _} [Complexity.Encoding β Memory] {f: α → β} {tp: TracedProgram}
 variable {γ: Type _} {δ: Type _} [Complexity.Encoding γ Memory] [Complexity.Encoding δ Memory] {fs: γ → δ} [Complexity.Computable Encoding.Model fs] [Complexity Encoding.Model fs]
 
-inductive CostedProgram: TracedProgram f → Type _
-| exit: CostedProgram .exit
-| op (inst: OpInstruction) {tp: TracedProgram f} (next: CostedProgram tp): CostedProgram (.op inst tp)
-| branch (inst: BranchInstruction) {tp: Bool → TracedProgram f} (pos: (b: Bool) → CostedProgram (tp b)): CostedProgram (.branch inst tp)
+inductive CostedProgram
+| exit
+| op (inst: OpInstruction) (next: CostedProgram)
+| branch (inst: BranchInstruction) (next: (b: Bool) → CostedProgram)
 | subroutine (dst src: Source) {γ: Type _} {δ: Type _} [Complexity.Encoding γ Memory] [Complexity.Encoding δ Memory]
-  {fs: γ → δ} [Complexity.Computable Encoding.Model fs] [Complexity Encoding.Model fs] {tp: TracedProgram f} (next: CostedProgram tp): CostedProgram (.subroutine dst src fs tp)
-| recurse (dst src: Source) {tp: TracedProgram f} (next: CostedProgram tp): CostedProgram (.recurse dst src tp)
+  (fs: γ → δ) [Complexity.Computable Encoding.Model fs] [Complexity Encoding.Model fs] (next: CostedProgram)
+| recurse (dst src: Source) (next: CostedProgram)
 
-class WithCost (tp: TracedProgram f) where
-  cost: CostedProgram tp
 
-instance: WithCost (f := f) .exit := ⟨ .exit ⟩
-instance [next: WithCost tp]: WithCost (f := f) (.op inst tp) := ⟨ .op inst next.cost ⟩
+namespace CostedProgram
 
-def timeCost {tp: TracedProgram f} (h: tp.sound size): Complexity.CostFunction α ℕ :=
-  λ a ↦ Program.timeCost _ (tp.halts h a)
+@[match_pattern] def subroutine' (dst src: Source) {γ: Type _} (_hγ: Complexity.Encoding γ Memory) {δ: Type _} (_hδ: Complexity.Encoding δ Memory)
+    (fs: γ → δ) (_h: Complexity.Computable Encoding.Model fs) (_h': Complexity Encoding.Model fs) (next: CostedProgram): CostedProgram :=
+  subroutine dst src fs next
 
-def localTimeCostInternal: {tp: TracedProgram f} → {fm: α → Option Memory} → (h: tp.soundInternal' size fm) → Complexity.CostFunction α ℕ
-| .exit, fm, _ => (1:Complexity.CostFunction Memory ℕ).flatMap fm
-| .op _ _, fm, h => localTimeCostInternal (TracedProgram.soundInternal'_op_next h) + (1:Complexity.CostFunction Memory ℕ).flatMap fm
-| .branch _ _, fm, h => localTimeCostInternal (TracedProgram.soundInternal'_branch_next_true h) + localTimeCostInternal (TracedProgram.soundInternal'_branch_next_false h) + (1:Complexity.CostFunction Memory ℕ).flatMap fm
-| .subroutine' _ _ _ _ _ _ _, fm, h => localTimeCostInternal (TracedProgram.soundInternal'_subroutine_next h) + (1:Complexity.CostFunction Memory ℕ).flatMap fm
-| .recurse _ _ _, fm, h => localTimeCostInternal (TracedProgram.soundInternal'_recurse_next h) + (1:Complexity.CostFunction Memory ℕ).flatMap fm
+def toTracedProgram: CostedProgram → TracedProgram
+| .exit => .exit
+| .op inst next => .op inst next.toTracedProgram
+| .branch inst next => .branch inst (λ b ↦ (next b).toTracedProgram)
+| .subroutine' dst src _ _ fs _ _ next => .subroutine dst src fs next.toTracedProgram
+| .recurse dst src next => .recurse dst src next.toTracedProgram
 
-theorem localTimeCostInternal_le_size: {tp: TracedProgram f} → (h: tp.soundInternal' size fm) →
-  ∀ a, localTimeCostInternal h a ≤ tp.toProgram.size
-| .exit, _, _ => Complexity.CostFunction.nat_flatMap_le_nat _ _ _
-| .op _ _, _, _ => add_le_add
-  (localTimeCostInternal_le_size _ _)
-  (Complexity.CostFunction.nat_flatMap_le_nat _ _ _)
-| .branch _ _, _, _ => add_le_add (add_le_add
-  (localTimeCostInternal_le_size _ _)
-  (localTimeCostInternal_le_size _ _))
-  (Complexity.CostFunction.nat_flatMap_le_nat _ _ _)
-| .subroutine' _ _ _ _ _ _ _, _, _ => add_le_add
-  (le_add_left (localTimeCostInternal_le_size _ _))
-  (Complexity.CostFunction.nat_flatMap_le_nat _ _ _)
-| .recurse _ _ _, _, _ => add_le_add
-  (localTimeCostInternal_le_size _ _)
-  (Complexity.CostFunction.nat_flatMap_le_nat _ _ _)
+end CostedProgram
 
-def localTimeCost (h: tp.sound size): Complexity.CostFunction α ℕ := localTimeCostInternal (TracedProgram.soundInternal'_of_sound h)
+class HasCostedProgram (p: Program) extends HasTracedProgram p where
+  costedProgram: CostedProgram
+  costedProgramMatches: costedProgram.toTracedProgram = tracedProgram
 
-def localTimeCost_O1 (h: tp.sound size): Complexity.O (localTimeCost h) = Complexity.O (1) :=
-  flip le_antisymm (Complexity.Asymptotic.o1_le _) ⟨_, le_add_left (localTimeCostInternal_le_size _)⟩
+-- class WithCost (tp: TracedProgram f) where
+--   cost: CostedProgram tp
 
-def subroutineTimeCostInternal: {tp: TracedProgram f} → CostedProgram tp → (h: tp.soundInternal' size fm) → Complexity.CostFunction α ℕ
-| _, .exit, _ => 0
-| _, .op _ next, h => subroutineTimeCostInternal next (TracedProgram.soundInternal'_op_next h)
-| _, .branch _ next, h =>
-  subroutineTimeCostInternal (next true) (TracedProgram.soundInternal'_branch_next_true h) +
-  subroutineTimeCostInternal (next false) (TracedProgram.soundInternal'_branch_next_false h)
-| _, @CostedProgram.subroutine _ _ _ _ _ _ _ _ _ _ _ _ _ hcost _ next, h =>
-  subroutineTimeCostInternal next (TracedProgram.soundInternal'_subroutine_next h) +
-  hcost.cost.flatMap (TracedProgram.soundInternal'_subroutine_arg h)
-| _, .recurse _ _ next, h => subroutineTimeCostInternal next (TracedProgram.soundInternal'_recurse_next h)
+-- instance: WithCost (f := f) .exit := ⟨ .exit ⟩
+-- instance [next: WithCost tp]: WithCost (f := f) (.op inst tp) := ⟨ .op inst next.cost ⟩
 
-def subroutineTimeCost {tp: TracedProgram f} [hc: WithCost tp] (h: tp.sound size): Complexity.CostFunction α ℕ :=
-  subroutineTimeCostInternal hc.cost (TracedProgram.soundInternal'_of_sound h)
+-- def timeCost {tp: TracedProgram f} (h: tp.sound size): Complexity.CostFunction α ℕ :=
+--   λ a ↦ Program.timeCost _ (tp.halts h a)
 
-def recurseTimeCostInternal {tp: TracedProgram f} (h: tp.sound size): {curr: TracedProgram f} → (hc: TracedProgram.soundInternal' size curr fm) → Complexity.CostFunction α ℕ
-| .exit, _ => 0
-| .op _ _, hc => recurseTimeCostInternal h (TracedProgram.soundInternal'_op_next hc)
-| .branch _ _, hc => recurseTimeCostInternal h (TracedProgram.soundInternal'_branch_next_true hc) + recurseTimeCostInternal h (TracedProgram.soundInternal'_branch_next_false hc)
-| .subroutine' _ _ _ _ _ _ _, hc => recurseTimeCostInternal h (TracedProgram.soundInternal'_subroutine_next hc)
-| .recurse _ _ _, hc => recurseTimeCostInternal h (TracedProgram.soundInternal'_recurse_next hc) + (timeCost h).flatMap (TracedProgram.soundInternal'_recurse_arg hc)
+-- def localTimeCostInternal: {tp: TracedProgram f} → {fm: α → Option Memory} → (h: tp.soundInternal' size fm) → Complexity.CostFunction α ℕ
+-- | .exit, fm, _ => (1:Complexity.CostFunction Memory ℕ).flatMap fm
+-- | .op _ _, fm, h => localTimeCostInternal (TracedProgram.soundInternal'_op_next h) + (1:Complexity.CostFunction Memory ℕ).flatMap fm
+-- | .branch _ _, fm, h => localTimeCostInternal (TracedProgram.soundInternal'_branch_next_true h) + localTimeCostInternal (TracedProgram.soundInternal'_branch_next_false h) + (1:Complexity.CostFunction Memory ℕ).flatMap fm
+-- | .subroutine' _ _ _ _ _ _ _, fm, h => localTimeCostInternal (TracedProgram.soundInternal'_subroutine_next h) + (1:Complexity.CostFunction Memory ℕ).flatMap fm
+-- | .recurse _ _ _, fm, h => localTimeCostInternal (TracedProgram.soundInternal'_recurse_next h) + (1:Complexity.CostFunction Memory ℕ).flatMap fm
 
-def recurseTimeCost (h: tp.sound size): Complexity.CostFunction α ℕ := recurseTimeCostInternal h (TracedProgram.soundInternal'_of_sound  h)
+-- theorem localTimeCostInternal_le_size: {tp: TracedProgram f} → (h: tp.soundInternal' size fm) →
+--   ∀ a, localTimeCostInternal h a ≤ tp.toProgram.size
+-- | .exit, _, _ => Complexity.CostFunction.nat_flatMap_le_nat _ _ _
+-- | .op _ _, _, _ => add_le_add
+--   (localTimeCostInternal_le_size _ _)
+--   (Complexity.CostFunction.nat_flatMap_le_nat _ _ _)
+-- | .branch _ _, _, _ => add_le_add (add_le_add
+--   (localTimeCostInternal_le_size _ _)
+--   (localTimeCostInternal_le_size _ _))
+--   (Complexity.CostFunction.nat_flatMap_le_nat _ _ _)
+-- | .subroutine' _ _ _ _ _ _ _, _, _ => add_le_add
+--   (le_add_left (localTimeCostInternal_le_size _ _))
+--   (Complexity.CostFunction.nat_flatMap_le_nat _ _ _)
+-- | .recurse _ _ _, _, _ => add_le_add
+--   (localTimeCostInternal_le_size _ _)
+--   (Complexity.CostFunction.nat_flatMap_le_nat _ _ _)
 
-theorem recurseTimeCostInternal_leaf {tp: TracedProgram f} (h: tp.sound size):
-    {curr: TracedProgram f} → (hc: TracedProgram.soundInternal' size curr fm) →
-    {a : α} → size a = 0 → recurseTimeCostInternal h hc a = 0
-| .exit, _, _, _ => rfl
-| .op _ next, _, _, hsize => recurseTimeCostInternal_leaf (curr := next) h _ hsize
-| .branch _ _, _, _, hsize =>
-  Nat.add_eq_zero_iff.mpr ⟨
-      recurseTimeCostInternal_leaf _ _ hsize,
-      recurseTimeCostInternal_leaf _ _ hsize ⟩
-| .subroutine' _ _ _ _ _ _ next, _, _, hsize => recurseTimeCostInternal_leaf (curr := next) h _ hsize
-| .recurse _ _ _, hc, _, hsize => Nat.add_eq_zero_iff.mpr ⟨
-    recurseTimeCostInternal_leaf _ _ hsize,
-    Complexity.CostFunction.flatMap_none
-      (Option.bind_of_none (Option.Forall_false (hc.right.left _) λ _ hm ↦
-        (Option.Exists_exists hm).elim λ _ ha ↦
-          Nat.not_lt_zero _ (Nat.lt_of_lt_of_eq ha.right hsize))) _ ⟩
+-- -- def localTimeCost (h: tp.sound size): Complexity.CostFunction α ℕ := localTimeCostInternal (TracedProgram.soundInternal'_of_sound h)
 
-theorem recurseTimeCostInternal_zero {tp: TracedProgram f} (h: tp.sound λ _ ↦ 0):
-  recurseTimeCost h = 0 := funext λ _ ↦ recurseTimeCostInternal_leaf h _ rfl
+-- -- def localTimeCost_O1 (h: tp.sound size): Complexity.O (localTimeCost h) = Complexity.O (1) :=
+-- --   flip le_antisymm (Complexity.Asymptotic.o1_le _) ⟨_, le_add_left (localTimeCostInternal_le_size _)⟩
 
-theorem splitTimeCostInternal {tp: TracedProgram f} (hp: tp.sound size): {curr: TracedProgram f} → (hc: CostedProgram curr) → {fm: α → Option Memory} → (h: curr.soundInternal' size fm) →
-    ∀ a, Option.Forall (λ m ↦ Stack.hasTimeCost
-      (.execution ⟨m, curr.toProgram, tp.toProgram⟩ [])
-      ((subroutineTimeCostInternal hc h + recurseTimeCostInternal hp h + localTimeCostInternal h) a)) (fm a)
-| _, .exit, fm, h, a =>
-  Option.Forall_forall λ _ hm ↦ ⟨_, Stack.istep_result_le (le_add_left (le_of_eq (Eq.symm (Complexity.CostFunction.flatMap_some hm _)))) rfl⟩
-| _, .op inst next, fm, h, a => by
-  apply Option.Forall_forall
-  intro m hm
-  -- apply Stack.hasTimeCost_step
-  sorry
-| _, _, _, _, _ => sorry
+-- def subroutineTimeCostInternal: {tp: TracedProgram f} → CostedProgram tp → (h: tp.soundInternal' size fm) → Complexity.CostFunction α ℕ
+-- | _, .exit, _ => 0
+-- | _, .op _ next, h => subroutineTimeCostInternal next (TracedProgram.soundInternal'_op_next h)
+-- | _, .branch _ next, h =>
+--   subroutineTimeCostInternal (next true) (TracedProgram.soundInternal'_branch_next_true h) +
+--   subroutineTimeCostInternal (next false) (TracedProgram.soundInternal'_branch_next_false h)
+-- | _, @CostedProgram.subroutine _ _ _ _ _ _ _ _ _ _ _ _ _ hcost _ next, h =>
+--   subroutineTimeCostInternal next (TracedProgram.soundInternal'_subroutine_next h) +
+--   hcost.cost.flatMap (TracedProgram.soundInternal'_subroutine_arg h)
+-- | _, .recurse _ _ next, h => subroutineTimeCostInternal next (TracedProgram.soundInternal'_recurse_next h)
+
+-- -- def subroutineTimeCost {tp: TracedProgram f} [hc: WithCost tp] (h: tp.sound size): Complexity.CostFunction α ℕ :=
+-- --   subroutineTimeCostInternal hc.cost (TracedProgram.soundInternal'_of_sound h)
+
+-- def recurseTimeCostInternal {tp: TracedProgram f} (h: tp.sound size): {curr: TracedProgram f} → (hc: TracedProgram.soundInternal' size curr fm) → Complexity.CostFunction α ℕ
+-- | .exit, _ => 0
+-- | .op _ _, hc => recurseTimeCostInternal h (TracedProgram.soundInternal'_op_next hc)
+-- | .branch _ _, hc => recurseTimeCostInternal h (TracedProgram.soundInternal'_branch_next_true hc) + recurseTimeCostInternal h (TracedProgram.soundInternal'_branch_next_false hc)
+-- | .subroutine' _ _ _ _ _ _ _, hc => recurseTimeCostInternal h (TracedProgram.soundInternal'_subroutine_next hc)
+-- | .recurse _ _ _, hc => recurseTimeCostInternal h (TracedProgram.soundInternal'_recurse_next hc) + (timeCost h).flatMap (TracedProgram.soundInternal'_recurse_arg hc)
+
+-- def recurseTimeCost (h: tp.sound size): Complexity.CostFunction α ℕ := recurseTimeCostInternal h (TracedProgram.soundInternal'_of_sound  h)
+
+-- theorem recurseTimeCostInternal_leaf {tp: TracedProgram f} (h: tp.sound size):
+--     {curr: TracedProgram f} → (hc: TracedProgram.soundInternal' size curr fm) →
+--     {a : α} → size a = 0 → recurseTimeCostInternal h hc a = 0
+-- | .exit, _, _, _ => rfl
+-- | .op _ next, _, _, hsize => recurseTimeCostInternal_leaf (curr := next) h _ hsize
+-- | .branch _ _, _, _, hsize =>
+--   Nat.add_eq_zero_iff.mpr ⟨
+--       recurseTimeCostInternal_leaf _ _ hsize,
+--       recurseTimeCostInternal_leaf _ _ hsize ⟩
+-- | .subroutine' _ _ _ _ _ _ next, _, _, hsize => recurseTimeCostInternal_leaf (curr := next) h _ hsize
+-- | .recurse _ _ _, hc, _, hsize => Nat.add_eq_zero_iff.mpr ⟨
+--     recurseTimeCostInternal_leaf _ _ hsize,
+--     Complexity.CostFunction.flatMap_none
+--       (Option.bind_of_none (Option.Forall_false (hc.right.left _) λ _ hm ↦
+--         (Option.Exists_exists hm).elim λ _ ha ↦
+--           Nat.not_lt_zero _ (Nat.lt_of_lt_of_eq ha.right hsize))) _ ⟩
+
+-- theorem recurseTimeCostInternal_zero {tp: TracedProgram f} (h: tp.sound λ _ ↦ 0):
+--   recurseTimeCost h = 0 := funext λ _ ↦ recurseTimeCostInternal_leaf h _ rfl
+
+-- theorem splitTimeCostInternal {tp: TracedProgram f} (hp: tp.sound size): {curr: TracedProgram f} → (hc: CostedProgram curr) → {fm: α → Option Memory} → (h: curr.soundInternal' size fm) →
+--     ∀ a, Option.Forall (λ m ↦ Stack.hasTimeCost
+--       (.execution ⟨m, curr.toProgram, tp.toProgram⟩ [])
+--       ((subroutineTimeCostInternal hc h + recurseTimeCostInternal hp h + localTimeCostInternal h) a)) (fm a)
+-- | _, .exit, fm, h, a =>
+--   Option.Forall_forall λ _ hm ↦ ⟨_, Stack.istep_result_le (le_add_left (le_of_eq (Eq.symm (Complexity.CostFunction.flatMap_some hm _)))) rfl⟩
+-- | _, .op inst next, fm, h, a => by
+--   apply Option.Forall_forall
+--   intro m hm
+--   apply Stack.hasTimeCost_of_step_le_succ _
+--   have hx := Option.Forall_of_some hm (Option.Forall_of_map (splitTimeCostInternal hp (hc := next) h a))
+--   exact hx
+--   apply le_of_le_of_eq _
+--   apply Nat.add_assoc _ _ _
+--   exact add_le_add (le_refl _) (le_of_eq (Eq.symm (Complexity.CostFunction.flatMap_some hm _)))
+-- | _, .branch inst next, fm, h, a => by
+--   apply Option.Forall_forall
+--   intro m hm
+--   match hi:inst.apply m with
+--   | true =>
+--     apply Stack.hasTimeCost_of_step_le_succ _
+--     have hx := hm ▸ splitTimeCostInternal hp (hc := (next true)) h.left a
+--     simp only [Option.filter, hm, hi, Option.Forall, Function.comp] at hx
+--     apply Option.Forall_of_some
+--     exact hm
+--   | false => sorry
+
+
+-- | _, _, _, _, _ => sorry
 
 
 end HMem.Trace
