HMem/Trace/Sound.lean
@@ -1,130 +1,97 @@
 import HMem.Trace.TracedProgram
 
-def Option.Forall (P: α → Prop): Option α → Prop
-| some a => P a
-| none => True
+@[simp] theorem Option.filter_none : Option.filter f none = none := rfl
 
-theorem Option.Forall_imp: {o: Option α} → Option.Forall P o → (∀ a, P a → Q a) → Option.Forall Q o
-| some _, hP, h => h _ hP
-| none, _, _ => trivial
+@[simp] theorem Option.filter_eq_some': {x: Option α} → x.filter f = some b ↔ x = some b ∧ f b
+| .none => ⟨ flip absurd Option.noConfusion, And.left ⟩
+| .some b => by simpa [Option.filter, And.comm (a := Eq b _)] using λ heq ↦ heq ▸ ⟨id, id⟩
 
-theorem Option.Forall_forall: {o: Option α} → (∀ a, o = some a → P a) → Option.Forall P o
-| some _, h => h _ rfl
-| none, _ => trivial
+theorem Option.forall_mem_filter {f : α → Bool} {o : Option α} {p : α → Prop} :
+  (∀ y ∈ o.filter f, p y) ↔ ∀ x ∈ o, f x → p x := by simp
 
-theorem Option.Forall_map: {o: Option α} → Option.Forall P (Option.map f o) = Option.Forall (P ∘ f) o
-| some _ => rfl
-| none => rfl
+theorem Option.mem_filter_of_mem {f : α → Bool} {o : Option α}
+    (hmem: x ∈ o) (hf: f x): x ∈ o.filter f := Option.filter_eq_some'.mpr ⟨hmem, hf⟩
 
-theorem Option.Forall_of_map (h: Option.Forall P (Option.map f o)): Option.Forall (P ∘ f) o :=
-  Option.Forall_map ▸ h
+theorem Option.forall_mem_bind {f : α → Option β} {o : Option α} {p : β → Prop}:
+  (∀ y ∈ Option.bind o f, p y) ↔ ∀ x ∈ o, ∀ y ∈ f x, p y := by
+    simpa using ⟨ λ h _ hx _ ↦ h _ _ hx, λ h _ _ hx ↦ h _ hx _ ⟩
 
-theorem Option.Forall_bind: {o: Option α} → Option.Forall P (Option.bind o f) = Option.Forall (Option.Forall P ∘ f) o
-| some _ => rfl
-| none => rfl
+theorem Option.mem_bind_of_mem {f : α → Option β} {o : Option α}
+    (ha: a ∈ o) (hf: b ∈ f a): b ∈ o.bind f := (congrArg₂ _ ha rfl).trans hf
 
-theorem Option.Forall_filter: {o: Option α} → Option.Forall P (Option.filter f o) = Option.Forall (λ a ↦ f a → P a) o
-| some a => if h:f a
-  then (congrArg (Forall P) (if_pos h)).trans (iff_iff_eq.mp ⟨ λ hf _ ↦ hf, λ hf ↦ hf h ⟩)
-  else (congrArg (Forall P) (if_neg h)).trans (eq_true (flip absurd h)).symm
-| none => rfl
-
-theorem Option.Forall_some_eq (h: o = Option.some a): Option.Forall P o = P a := h ▸ rfl
-theorem Option.Forall_of_some (h: o = Option.some a): Option.Forall P o → P a := Forall_some_eq h ▸ id
-theorem Option.Forall_some (h: o = Option.some a): P a → Option.Forall P o := Forall_some_eq h ▸ id
-theorem Option.Forall_isSome: {o: Option α} → (h: Option.isSome o) → P (o.get h) → Option.Forall P o
-| some _, _ => id
-| none, h => absurd h Bool.noConfusion
-
-theorem Option.Forall_none (h: o = none): Option.Forall P o := h ▸ trivial
-
-def Option.Exists (P: α → Prop): Option α → Prop
-| some a => P a
-| none => False
-
-
-def Option.Exists_of_isSome: {o: Option α} → (hs: o.isSome) → P (o.get hs) → Option.Exists P o
-| some _, _, hP => hP
-| none, hs, _ => absurd hs Bool.noConfusion
-
-def Option.Exists_isSome: {o: Option α} → (hs: o.isSome) → Option.Exists P o → P (o.get hs)
-| some _, _, hP => hP
-| none, hs, _ => absurd hs Bool.noConfusion
-
-namespace HMem.Trace
-
-namespace TracedProgram
+namespace HMem
 variable {α: Type _} [Complexity.Encoding α Memory] {β: Type _} [Complexity.Encoding β Memory] {f: α → β}
+
+namespace Trace.TracedProgram
 variable {γ: Type _} {δ: Type _} [enγ: Complexity.Encoding γ Memory] [enδ: Complexity.Encoding δ Memory] {fs: γ → δ} [hc: Complexity.Computable Encoding.Model fs]
-def soundInternal (size: α → ℕ) (a: α): TracedProgram f → Memory → Prop
+
+def sound (f: α → β) (size: α → ℕ) (a: α): TracedProgram → Memory → Prop
 | exit, m => m = Complexity.encode (f a)
-| op inst next, m => next.soundInternal size a (inst.apply m)
-| branch inst next, m => (next (inst.apply m)).soundInternal size a m
+| op inst next, m => next.sound f size a (inst.apply m)
+| branch inst next, m => (next (inst.apply m)).sound f size a m
 | subroutine dst src func next, m =>
   ∃ arg,
     m.getms src = Complexity.encode arg ∧
-    next.soundInternal size a (m.setms dst (Complexity.encode (func arg)))
+    next.sound f size a (m.setms dst (Complexity.encode (func arg)))
 | recurse dst src next, m =>
   ∃ arg,
     m.getms src = Complexity.encode arg ∧
     size arg < size a ∧
-    next.soundInternal size a (m.setms dst (Complexity.encode (f arg)))
+    next.sound f size a (m.setms dst (Complexity.encode (f arg)))
 
-@[simp] def sound (tp: TracedProgram f) (size: α → ℕ): Prop := ∀ a, tp.soundInternal size a (Complexity.encode a)
+theorem sound_branch_eq (h: inst.apply m = b):
+    sound f size a (branch inst next) m = sound f size a (next b) m := h ▸ rfl
 
-theorem soundInternal_branch_eq (h: inst.apply m = b):
-    soundInternal size a (branch (f := f) inst next) m = soundInternal size a (next b) m := h ▸ rfl
-
-theorem soundInternal_subroutine_some (h: soundInternal size a (subroutine (f := f) dst src fs next) m):
+theorem sound_subroutine_some (h: sound f size a (subroutine dst src fs next) m):
     Option.isSome (Complexity.decode γ (m.getms src)) :=
   h.elim λ | arg, ⟨h, _⟩ => h ▸ Complexity.decode_inv arg (Data := Memory) ▸ rfl
 
-theorem soundInternal_recurse_some (h: soundInternal size a (recurse (f := f) dst src next) m):
+theorem sound_recurse_some (h: sound f size a (recurse dst src next) m):
     Option.isSome (Complexity.decode α (m.getms src)) :=
   h.elim λ | arg, ⟨h, _, _⟩ => h ▸ Complexity.decode_inv arg (Data := Memory) ▸ rfl
 
-@[simp] theorem soundInternal_exit: (soundInternal size a (exit (f := f)) m) = (m = Complexity.encode (f a)) := rfl
-@[simp] theorem soundInternal_op: (soundInternal size a (op (f := f) inst next) m) = (next.soundInternal size a (inst.apply m)) := rfl
-theorem soundInternal_op_next: soundInternal size a (op (f := f) inst next) m → next.soundInternal size a (inst.apply m) := id
-@[simp] theorem soundInternal_branch: (soundInternal size a (branch (f := f) inst next) m) = ((next (inst.apply m)).soundInternal size a m) := rfl
-theorem soundInternal_branch_next: soundInternal size a (branch (f := f) inst next) m → (next (inst.apply m)).soundInternal size a m := id
-@[simp] theorem soundInternal_subroutine: (soundInternal size a (subroutine (f := f) dst src fs next) m) = (∃ arg,
+@[simp] theorem sound_exit: (sound f size a exit m) = (m = Complexity.encode (f a)) := rfl
+@[simp] theorem sound_op: (sound f size a (op inst next) m) = (next.sound f size a (inst.apply m)) := rfl
+theorem sound_op_next: sound f size a (op inst next) m → next.sound f size a (inst.apply m) := id
+@[simp] theorem sound_branch: (sound f size a (branch inst next) m) = ((next (inst.apply m)).sound f size a m) := rfl
+theorem sound_branch_next: sound f size a (branch inst next) m → (next (inst.apply m)).sound f size a m := id
+@[simp] theorem sound_subroutine: (sound f size a (subroutine dst src fs next) m) = (∃ arg,
     Complexity.decode γ (m.getms src) = some arg ∧
     m.getms src = Complexity.encode arg ∧
-    next.soundInternal size a (m.setms dst (Complexity.encode (fs arg)))) :=
+    next.sound f size a (m.setms dst (Complexity.encode (fs arg)))) :=
   iff_iff_eq.mp (exists_congr λ _ ↦ ⟨ λ h ↦ ⟨ h.left ▸ Complexity.decode_inv _, h ⟩, And.right ⟩)
-theorem soundInternal_subroutine_arg (h: soundInternal size a (subroutine (f := f) dst src fs next) m):
-    m.getms src = Complexity.encode (Option.get _ (soundInternal_subroutine_some h)) :=
+theorem sound_subroutine_arg (h: sound f size a (subroutine dst src fs next) m):
+    m.getms src = Complexity.encode (Option.get _ (sound_subroutine_some h)) :=
   h.elim λ | _, ⟨hm, _⟩ => by simp only [hm, Complexity.decode_inv, Option.get_some]
-theorem soundInternal_subroutine_next (h: soundInternal size a (subroutine (f := f) dst src fs next) m):
-    next.soundInternal size a (m.setms dst (Complexity.encode (fs (Option.get _ (soundInternal_subroutine_some h))))) :=
+theorem sound_subroutine_next (h: sound f size a (subroutine dst src fs next) m):
+    next.sound f size a (m.setms dst (Complexity.encode (fs (Option.get _ (sound_subroutine_some h))))) :=
   h.elim λ | _, ⟨hm, h⟩ => by simpa only [hm, Complexity.decode_inv, Option.get_some] using h
 
-@[simp] theorem soundInternal_recurse: (soundInternal size a (recurse (f := f) dst src next) m) = (∃ arg,
+@[simp] theorem sound_recurse: (sound f size a (recurse dst src next) m) = (∃ arg,
     Complexity.decode α (m.getms src) = some arg ∧
     m.getms src = Complexity.encode arg ∧
     size arg < size a ∧
-    next.soundInternal size a (m.setms dst (Complexity.encode (f arg)))) :=
+    next.sound f size a (m.setms dst (Complexity.encode (f arg)))) :=
   iff_iff_eq.mp (exists_congr λ _ ↦ ⟨ λ h ↦ ⟨ h.left ▸ Complexity.decode_inv _, h ⟩, And.right ⟩)
-theorem soundInternal_recurse_arg (h: soundInternal size a (recurse (f := f) dst src next) m):
-    m.getms src = Complexity.encode (Option.get _ (soundInternal_recurse_some h)) :=
+theorem sound_recurse_arg (h: sound f size a (recurse dst src next) m):
+    m.getms src = Complexity.encode (Option.get _ (sound_recurse_some h)) :=
   h.elim λ | _, ⟨hm, _, _⟩ => by simp only [hm, Complexity.decode_inv, Option.get_some]
-theorem soundInternal_recurse_size (h: soundInternal size a (recurse (f := f) dst src next) m):
-    size (Option.get _ (soundInternal_recurse_some h)) < size a :=
+theorem sound_recurse_size (h: sound f size a (recurse dst src next) m):
+    size (Option.get _ (sound_recurse_some h)) < size a :=
   h.elim λ | _, ⟨hm, hs, _⟩ => by simpa only [hm, Complexity.decode_inv, Option.get_some] using hs
-theorem soundInternal_recurse_next (h: soundInternal size a (recurse (f := f) dst src next) m):
-    next.soundInternal size a (m.setms dst (Complexity.encode (f (Option.get _ (soundInternal_recurse_some h))))) :=
+theorem sound_recurse_next (h: sound f size a (recurse dst src next) m):
+    next.sound f size a (m.setms dst (Complexity.encode (f (Option.get _ (sound_recurse_some h))))) :=
   h.elim λ | _, ⟨hm, _, h⟩ => by simpa only [hm, Complexity.decode_inv, Option.get_some] using h
 
 theorem hasResultInternal
     {size: α → ℕ}
     {a: α}
-    {tp: TracedProgram f}
+    {tp: TracedProgram}
     (ih: ∀ arg, size arg < size a →
       tp.toProgram.hasResult (Complexity.encode arg) (Complexity.encode (f arg))):
-    {current: TracedProgram f} →
+    {current: TracedProgram} →
     {m: Memory} →
-    (h: soundInternal size a current m) →
+    (h: sound f size a current m) →
     Stack.hasResult (.execution ⟨m, current.toProgram, tp.toProgram⟩ []) (Complexity.encode (f a))
 | .exit, _, h => ⟨1, congrArg Stack.result h⟩
 | .op _ _, _, h => Stack.hasResult_of_step (hasResultInternal ih h)
@@ -138,163 +105,153 @@ theorem hasResultInternal
     (hm.symm ▸ ih _ hsize)
     (hasResultInternal ih h)
 
-theorem hasResultHelper
-    {tp: TracedProgram f} {size: α → ℕ} (h: tp.sound size) (n: ℕ):
-    ∀ a, n = size a → tp.toProgram.hasResult (Complexity.encode a) (Complexity.encode (f a)) :=
-  n.strong_induction_on λ _ ih _ ha ↦
-    hasResultInternal
-      (λ _ harg ↦ ih _ (ha ▸ harg) _ rfl)
-      (h _)
-
-theorem hasResult {tp: TracedProgram f} {size: α → ℕ} (h: tp.sound size) (a: α):
-    tp.toProgram.hasResult (Complexity.encode a) (Complexity.encode (f a)) :=
-  hasResultHelper h _ a rfl
-
-theorem halts {tp: TracedProgram f} {size: α → ℕ} (h: tp.sound size) (a: α):
-    tp.toProgram.haltsOn (Complexity.encode a) :=
-  (hasResult h a).elim λ _ hm => ⟨(_, _), hm⟩
-
-def soundInternal' (size: α → ℕ): TracedProgram f → (α → Option Memory) → Prop
-| exit, fm => ∀ a, (fm a).Forall (λ m ↦ m = Complexity.encode (f a))
-| op inst next, fm => next.soundInternal' size (Option.map inst.apply ∘ fm)
+def sound' (f: α → β) (size: α → ℕ): TracedProgram → (α → Option Memory) → Prop
+| exit, fm => ∀ a, ∀ m ∈ (fm a), m = Complexity.encode (f a)
+| op inst next, fm => next.sound' f size (Option.map inst.apply ∘ fm)
 | branch inst next, fm =>
-  (next true).soundInternal' size (Option.filter inst.apply ∘ fm) ∧
-  (next false).soundInternal' size (Option.filter (Bool.not ∘ inst.apply) ∘ fm)
+  (next true).sound' f size (Option.filter inst.apply ∘ fm) ∧
+  (next false).sound' f size (Option.filter (Bool.not ∘ inst.apply) ∘ fm)
 | subroutine' dst src enγ _ fs _ next, fm =>
-  (∀ a, (fm a).Forall (λ m ↦ ∃ (hm: Option.isSome (Complexity.decode (en := enγ) (m.getms src))), m.getms src = Complexity.encode (Option.get _ hm))) ∧
-  next.soundInternal' size (flip Option.bind
+  (∀ a, ∀ m ∈ (fm a), ∃ (hm: Option.isSome (Complexity.decode (en := enγ) (m.getms src))), m.getms src = Complexity.encode (Option.get _ hm)) ∧
+  next.sound' f size (flip Option.bind
     (λ m ↦ (Complexity.decode _ (m.getms src)).map
       (m.setms dst ∘ Complexity.encode ∘ fs)) ∘
     fm)
 | recurse dst src next, fm =>
-  (∀ a, (fm a).Forall (λ m ↦ ∃ (hm: Option.isSome (Complexity.decode α (m.getms src))), m.getms src = Complexity.encode (Option.get _ hm))) ∧
-  (∀ a, (fm a).Forall (λ m ↦ (Complexity.decode α (m.getms src)).Exists (λ arg ↦ size arg < size a))) ∧
-  next.soundInternal' size (flip Option.bind
+  (∀ a, ∀ m ∈ (fm a), ∃ (hm: Option.isSome (Complexity.decode α (m.getms src))), m.getms src = Complexity.encode (Option.get _ hm)) ∧
+  (∀ a, ∀ m ∈ (fm a), ∃ arg ∈ Complexity.decode α (m.getms src), size arg < size a) ∧
+  next.sound' f size (flip Option.bind
     (λ m ↦ (Complexity.decode α (m.getms src)).map
       (m.setms dst ∘ Complexity.encode ∘ f)) ∘
     fm)
 
-theorem soundInternal'_op_next:
-    soundInternal' size (.op (f := f) inst next) fm → soundInternal' size next (Option.map inst.apply ∘ fm) := id
+theorem sound'_op_next:
+    sound' f size (.op inst next) fm → sound' f size next (Option.map inst.apply ∘ fm) := id
 
-theorem soundInternal'_branch_next_true:
-    soundInternal' size (.branch (f := f) inst next) fm →
-      (next true).soundInternal' size (Option.filter inst.apply ∘ fm) := And.left
+theorem sound'_branch_next_true:
+    sound' f size (.branch inst next) fm →
+      (next true).sound' f size (Option.filter inst.apply ∘ fm) := And.left
 
-theorem soundInternal'_branch_next_false:
-    soundInternal' size (.branch (f := f) inst next) fm →
-  (next false).soundInternal' size (Option.filter (Bool.not ∘ inst.apply) ∘ fm) := And.right
+theorem sound'_branch_next_false:
+    sound' f size (.branch inst next) fm →
+  (next false).sound' f size (Option.filter (Bool.not ∘ inst.apply) ∘ fm) := And.right
 
-@[simp] def soundInternal'_subroutine_arg (_: soundInternal' size (.subroutine (f := f) dst src fs next) fm): α → Option γ :=
+@[simp] def sound'_subroutine_arg (_: sound' f size (.subroutine dst src fs next) fm): α → Option γ :=
   flip Option.bind (Complexity.decode _ ∘ flip Memory.getms src) ∘ fm
 
-theorem soundInternal'_subroutine_next:
-    soundInternal' size (.subroutine (f := f) dst src fs next) fm →
-    soundInternal' size next (flip Option.bind
+theorem sound'_subroutine_next:
+    sound' f size (.subroutine dst src fs next) fm →
+    sound' f size next (flip Option.bind
       (λ m ↦ (Complexity.decode _ (m.getms src)).map
         (m.setms dst ∘ Complexity.encode ∘ fs)) ∘
       fm) := And.right
 
-@[simp] def soundInternal'_recurse_arg (_: soundInternal' size (.recurse (f := f) dst src next) fm): α → Option α :=
+@[simp] def sound'_recurse_arg (_: sound' f size (.recurse dst src next) fm): α → Option α :=
     flip Option.bind (Complexity.decode _ ∘ flip Memory.getms src) ∘ fm
 
-theorem soundInternal'_recurse_next:
-    soundInternal' size (.recurse (f := f) dst src next) fm →
-    soundInternal' size next (flip Option.bind
+theorem sound'_recurse_next:
+    sound' f size (.recurse dst src next) fm →
+    sound' f size next (flip Option.bind
       (λ m ↦ (Complexity.decode _ (m.getms src)).map
         (m.setms dst ∘ Complexity.encode ∘ f)) ∘
       fm) := And.right ∘ And.right
 
-theorem soundInternal'_of_soundInternal: {tp: TracedProgram f} → {fm: α → Option Memory} →
-    (∀ a, (fm a).Forall (soundInternal size a tp)) → soundInternal' size tp fm
+theorem sound'_of_sound: {tp: TracedProgram} → {fm: α → Option Memory} →
+    (∀ a, ∀ m ∈ (fm a), sound f size a tp m) → sound' f size tp fm
 | .exit, _, h => h
-| .op _ next, _, h =>
-  soundInternal'_of_soundInternal (tp := next)
-    λ _ ↦ Option.Forall_map.symm ▸ h _
+| .op _ next, _, h => sound'_of_sound (tp := next) (λ _ ↦ Option.forall_mem_map.mpr (h _))
 | .branch _ _, _, h => ⟨
-    soundInternal'_of_soundInternal λ _ ↦
-      Option.Forall_filter ▸
-      Option.Forall_imp (h _) ( λ _ h heq ↦ heq ▸ h),
-    soundInternal'_of_soundInternal λ _ ↦
-      Option.Forall_filter ▸
-      Option.Forall_imp (h _) (λ _ h heq ↦
-        (((Bool.not_not _).symm.trans (congrArg Bool.not heq)).trans Bool.not_true)
-          ▸ h)⟩
-| .subroutine' _ _ _ _ _ _ _, _, h => ⟨
-  λ _ ↦ Option.Forall_forall λ _ hm ↦
-    ⟨_, soundInternal_subroutine_arg (Option.Forall_of_some hm (h _))⟩,
-  soundInternal'_of_soundInternal λ _ ↦
-    Option.Forall_bind ▸
-    Option.Forall_imp (h _) (λ _ hm ↦
-      Function.comp_apply ▸
-      Option.Forall_map.symm ▸
-      Option.Forall_isSome
-        (soundInternal_subroutine_some hm)
-        (soundInternal_subroutine_next hm))⟩
-| .recurse _ _ _, _, h => ⟨
-  λ _ ↦ Option.Forall_forall λ _ hm ↦
-    ⟨_, soundInternal_recurse_arg (Option.Forall_of_some hm (h _))⟩,
-  λ _ ↦ Option.Forall_forall λ _ hm ↦
-    Option.Exists_of_isSome _ (soundInternal_recurse_size (Option.Forall_of_some hm (h _))),
-  soundInternal'_of_soundInternal λ _ ↦
-    Option.Forall_bind ▸
-    Option.Forall_imp (h _) (λ _ hm ↦
-      Function.comp_apply ▸
-      Option.Forall_map.symm ▸
-      Option.Forall_isSome
-        (soundInternal_recurse_some hm)
-        (soundInternal_recurse_next hm))⟩
+    sound'_of_sound λ _ ↦
+      Option.forall_mem_filter.mpr λ _ hm ht ↦
+        ht ▸ h _ _ hm,
+    sound'_of_sound λ _ ↦
+      Option.forall_mem_filter.mpr λ _ hm hf ↦
+        (Bool.not_not _).symm.trans ((congrArg Bool.not hf).trans Bool.not_true) ▸
+          h _ _ hm⟩
+| .subroutine' _ _ _ _ _ _ _, _, h =>
+  ⟨ λ _ _ hm ↦ ⟨_, sound_subroutine_arg (h _ _ hm)⟩,
+    sound'_of_sound λ _ ↦
+      Option.forall_mem_bind.mpr λ _ hm ↦
+        Option.forall_mem_map.mpr λ _ hc ↦
+          Option.get_of_mem _ hc ▸
+          sound_subroutine_next (h _ _ hm) ⟩
+| .recurse _ _ _, _, h =>
+  ⟨ λ _ _ hm ↦ ⟨_, sound_recurse_arg (h _ _ hm)⟩,
+    λ _ _ hm ↦ ⟨_, Option.get_mem _, sound_recurse_size (h _ _ hm)⟩,
+    sound'_of_sound λ _ ↦
+      Option.forall_mem_bind.mpr λ _ hm ↦
+        Option.forall_mem_map.mpr λ _ hc ↦
+          Option.get_of_mem _ hc ▸
+          sound_recurse_next (h _ _ hm) ⟩
 
-theorem soundInternal_of_soundInternal': {tp: TracedProgram f} → {fm: α → Option Memory} →
-    soundInternal' size tp fm → ∀ a, (fm a).Forall (soundInternal size a tp)
-| .exit, _, h, _ => h _
-| .op _ next, _, h, _ => Option.Forall_map ▸ soundInternal_of_soundInternal' (tp := next) h _
-| .branch inst _, _, h, _ => Option.Forall_forall λ m hm ↦ match hb: inst.apply m with
-  | true => soundInternal_branch_eq (f := f) hb ▸
-    (Option.Forall_of_some hm
-      (Option.Forall_filter ▸ soundInternal_of_soundInternal' h.left _))
-      hb
-  | false => soundInternal_branch_eq (f := f) hb ▸
-    (Option.Forall_of_some hm
-      (Option.Forall_filter ▸ soundInternal_of_soundInternal' h.right _))
-      (congrArg Bool.not hb)
-| .subroutine' _ _ _ _ _ _ _, _, h, _ =>
-  Option.Forall_forall λ _ hm ↦
-    (Option.Forall_of_some hm (h.left _)).elim λ hSome heq ↦
-    ⟨ _, heq, Option.Forall_of_some
-        ((congrArg₂ _ hm rfl).trans
-        (congrArg₂ Option.map rfl (Option.some_get hSome).symm))
-      (soundInternal_of_soundInternal' h.right _) ⟩
-| .recurse _ _ _, _, h, a =>
-  Option.Forall_forall λ _ hm ↦
-    (Option.Forall_of_some hm (h.left _)).elim λ hSome heq ↦ ⟨
-        Option.get _ hSome,
-        heq,
-        Option.Exists_isSome hSome (hm ▸ h.right.left a),
-        Option.Forall_of_some
-            ((congrArg₂ _ hm rfl).trans
-            (congrArg₂ Option.map rfl (Option.some_get hSome).symm))
-          (soundInternal_of_soundInternal' h.right.right _)
-      ⟩
+theorem sound_of_sound': {tp: TracedProgram} → {fm: α → Option Memory} →
+    sound' f size tp fm → ∀ a, ∀ m ∈ (fm a), sound f size a tp m
+| .exit, _, h, _, _, hm => h _ _ hm
+| .op _ next, _, h, _, _, hm =>
+  sound_of_sound' (tp := next) h _ _
+    (Option.mem_map_of_mem _ hm)
+| .branch inst _, _, h, _, m, hm =>
+  match hb:inst.apply m with
+  | true => sound_branch_eq (f := f) hb ▸
+    sound_of_sound' h.left _ _
+      (Option.mem_filter_of_mem hm hb)
+  | false => sound_branch_eq (f := f) hb ▸
+    sound_of_sound' h.right _ _
+      (Option.mem_filter_of_mem hm (congrArg Bool.not hb))
+| .subroutine' _ _ _ _ _ _ _, _, h, a, m, hm =>
+  (h.left a m hm).elim λ _ harg ↦
+    ⟨_, harg,
+      sound_of_sound' h.right _ _
+        (Option.mem_bind_of_mem hm
+          (Option.mem_map_of_mem _ (Option.get_mem _)))⟩
+| .recurse _ _ _, _, h, a, m, hm =>
+  (h.left a m hm).elim λ _ harg ↦
+    ⟨_, harg,
+      (h.right.left a m hm).elim λ _ hr ↦
+        lt_of_eq_of_lt (congrArg _ (Option.get_of_mem _ hr.left)) hr.right,
+      sound_of_sound' h.right.right _ _
+        (Option.mem_bind_of_mem hm
+          (Option.mem_map_of_mem _ (Option.get_mem _)))⟩
 
-theorem soundInternal_iff_soundInternal': soundInternal' (f := f) size tp fm ↔ ∀ a, (fm a).Forall (soundInternal size a tp) :=
-  ⟨ soundInternal_of_soundInternal', soundInternal'_of_soundInternal ⟩
+end Trace.TracedProgram
 
-theorem soundInternal'_def: soundInternal' (f := f) size tp fm = ∀ a, (fm a).Forall (soundInternal size a tp) :=
-  eq_iff_iff.mpr soundInternal_iff_soundInternal'
+namespace Program
 
-theorem soundInternal'_of_sound: sound (f := f) tp size → soundInternal' size tp (some ∘ Complexity.encode) :=
-  soundInternal'_def (f := f) ▸ id
 
-end TracedProgram
 
-class HasTrace {α: Type _} [Complexity.Encoding α Memory] {β: Type _} [Complexity.Encoding β Memory] (f: α → β) where
-  program: List (TracedProgram f → TracedProgram f)
+def sound (p: Program) [Trace.HasTracedProgram p] (f: α → β) (size: α → ℕ): Prop := ∀ a, p.traced.sound f size a (Complexity.encode a)
+
+
+theorem hasResult_of_soundHelper {p: Program} [Trace.HasTracedProgram p] {size: α → ℕ} (h: p.sound f size) (n: ℕ):
+    ∀ a, n = size a → p.hasResult (Complexity.encode a) (Complexity.encode (f a)) :=
+  p.tracedMatches ▸ n.strong_induction_on λ _ ih _ ha ↦
+    p.traced.hasResultInternal
+      (λ _ harg ↦ p.tracedMatches.symm ▸ ih _ (ha ▸ harg) _ rfl)
+      (h _)
+
+theorem hasResult_of_sound {p: Program} [Trace.HasTracedProgram p] {size: α → ℕ} (h: p.sound f size) (a: α):
+    p.hasResult (Complexity.encode a) (Complexity.encode (f a)) :=
+  p.hasResult_of_soundHelper h _ a rfl
+
+
+theorem halts_of_sound {p: Program} [Trace.HasTracedProgram p] {size: α → ℕ} (h: p.sound f size) (a: α):
+    p.haltsOn (Complexity.encode a) :=
+  (p.hasResult_of_sound h a).elim λ _ hm => ⟨(_, _), hm⟩
+
+class HasTrace (f: α → β) where
+  program: List (Program → Program)
+  hasTracedProgram: Trace.HasTracedProgram (Program.build program)
   size: α → ℕ
-  sound: (TracedProgram.build program).sound size
+  sound: (Program.build program).sound f size
+
+instance [tr: HasTrace f]: Trace.HasTracedProgram (Program.build tr.program) := tr.hasTracedProgram
 
 instance {α: Type _} [Complexity.Encoding α Memory] {β: Type _} [Complexity.Encoding β Memory] {f: α → β} [tr: HasTrace f]: Complexity.Computable Encoding.Model f where
-  program := (TracedProgram.build tr.program).toProgram
-  has_result := TracedProgram.hasResult tr.sound
+  program := .build tr.program
+  has_result := Program.hasResult_of_sound tr.sound
 
-end HMem.Trace
+end Program
+
+
+
+end HMem
