HMem/Trace/TracedProgram.lean
@@ -4,41 +4,51 @@ import HMem.Encoding.Basic
 namespace HMem
 namespace Trace
 
-inductive TracedProgram {α: Type _} [Complexity.Encoding α Memory] {β: Type _} [Complexity.Encoding β Memory] (f: α → β)
+inductive TracedProgram
 | exit
-| op (inst: OpInstruction) (next: TracedProgram f)
-| branch (inst: BranchInstruction) (next: Bool → TracedProgram f)
+| op (inst: OpInstruction) (next: TracedProgram)
+| branch (inst: BranchInstruction) (next: Bool → TracedProgram)
 | subroutine (dst src: Source) {γ: Type _} [enγ: Complexity.Encoding γ Memory] {δ: Type _} [enδ: Complexity.Encoding δ Memory]
-  (fs: γ → δ) [h: Complexity.Computable Encoding.Model fs] (next: TracedProgram f)
-| recurse (dst src: Source) (next: TracedProgram f)
+  (fs: γ → δ) [h: Complexity.Computable Encoding.Model fs] (next: TracedProgram)
+| recurse (dst src: Source) (next: TracedProgram)
 
 namespace TracedProgram
 variable {α: Type _} [Complexity.Encoding α Memory] {β: Type _} [Complexity.Encoding β Memory] {f: α → β}
 
-@[simp] def build: List (TracedProgram f → TracedProgram f) → TracedProgram f
+@[simp] def build: List (TracedProgram → TracedProgram) → TracedProgram
 | [] => .exit
 | p::ps => p (build ps)
 
-@[simp] def setv (dst: Source) (b: Bool): TracedProgram f → TracedProgram f := op (.vop (λ _ ↦ b) dst finZeroElim)
-@[simp] def setm (dst: Source) (src: Memory): TracedProgram f  → TracedProgram f := op (.const dst src)
-@[simp] def copyv (dst src: Source): TracedProgram f  → TracedProgram f := op (.vop (λ f ↦ f 0) dst (λ (_: Fin 1) ↦ src))
-@[simp] def copy (dst src: Source): TracedProgram f  → TracedProgram f := op (.mop .COPY dst src)
-@[simp] def move (dst src: Source): TracedProgram f  → TracedProgram f := op (.mop .MOVE dst src)
-@[simp] def swap (dst src: Source): TracedProgram f  → TracedProgram f := op (.mop .SWAP dst src)
-@[simp] def ifv (src: Source) (pos: List (TracedProgram f  → TracedProgram f)) (neg: TracedProgram f): TracedProgram f := branch (.ifTrue (λ f ↦ f 0) (λ (_: Fin 1) ↦ src)) (λ | true => build pos | false => neg)
+@[simp] def setv (dst: Source) (b: Bool): TracedProgram → TracedProgram := op (.vop (λ _ ↦ b) dst finZeroElim)
+@[simp] def setm (dst: Source) (src: Memory): TracedProgram  → TracedProgram := op (.const dst src)
+@[simp] def copyv (dst src: Source): TracedProgram  → TracedProgram := op (.vop (λ f ↦ f 0) dst (λ (_: Fin 1) ↦ src))
+@[simp] def copy (dst src: Source): TracedProgram  → TracedProgram := op (.mop .COPY dst src)
+@[simp] def move (dst src: Source): TracedProgram  → TracedProgram := op (.mop .MOVE dst src)
+@[simp] def swap (dst src: Source): TracedProgram  → TracedProgram := op (.mop .SWAP dst src)
+@[simp] def ifv (src: Source) (pos: List (TracedProgram  → TracedProgram)) (neg: TracedProgram): TracedProgram := branch (.ifTrue (λ f ↦ f 0) (λ (_: Fin 1) ↦ src)) (λ | true => build pos | false => neg)
 
 @[match_pattern] def subroutine' (dst src: Source) {γ: Type _} (_hγ: Complexity.Encoding γ Memory) {δ: Type _} (_hδ: Complexity.Encoding δ Memory)
-    (fs: γ → δ) (_h: Complexity.Computable Encoding.Model fs) (next: TracedProgram f): TracedProgram f :=
+    (fs: γ → δ) (_h: Complexity.Computable Encoding.Model fs) (next: TracedProgram): TracedProgram :=
   subroutine dst src fs next
 
-def toProgram: TracedProgram f → Program
+def toProgram: TracedProgram → Program
 | exit => .exit
 | op inst next => .op inst next.toProgram
 | branch inst next => .branch inst (λ b ↦ toProgram (next b))
 | subroutine dst src fs next => .subroutine dst src (Encoding.getProgram fs) next.toProgram
 | recurse dst src next => .recurse dst src next.toProgram
 
-
 end TracedProgram
+
+class HasTracedProgram (p: Program) where
+  tracedProgram: TracedProgram
+  tracedProgramMatches: tracedProgram.toProgram = p
+
 end Trace
+
+def Program.traced (p: Program) [htp: Trace.HasTracedProgram p]: Trace.TracedProgram := htp.tracedProgram
+
+@[simp] theorem Program.tracedMatches (p: Program) [Trace.HasTracedProgram p]:
+    p.traced.toProgram = p := Trace.HasTracedProgram.tracedProgramMatches
+
 end HMem
