HMem/Complexity/Basic.lean
@@ -8,9 +8,10 @@ import Complexity.Basic
 
 namespace HMem.Complexity
 
-instance [Complexity.Encoding α Memory]: Trace.HasTrace ↿(@List.cons α) where
-  program := [ .setv 0 true ]
-  size _ := 0
-  sound | (_, _) => by simp
+-- instance [Complexity.Encoding α Memory]: Program.HasTrace ↿(@List.cons α) where
+--   program := [ .setv 0 true ]
+--   hasTracedProgram := inferInstance
+--   size _ := 0
+--   sound | (_, _) => by simp
 
 end HMem.Complexity
