HMem/Complexity/Memory.lean
@@ -4,63 +4,63 @@ import HMem.Complexity.Basic
 import Complexity.Basic
 
 namespace HMem.Complexity
-instance: Trace.HasTrace Memory.getv where
-  program := [
-    .setm 1 0,
-    .setm 2 0
-  ]
-  size _ := 0
-  sound _ := by simp
+-- instance: Trace.HasTrace Memory.getv where
+--   program := [
+--     .setm 1 0,
+--     .setm 2 0
+--   ]
+--   size _ := 0
+--   sound _ := by simp
 
-instance: Trace.HasTrace ↿Memory.getm where
-  program := [ .move .nil (.imm false (.idx 2 0)) ]
-  size _ := 0
-  sound | (_, _) => by simp
+-- instance: Trace.HasTrace ↿Memory.getm where
+--   program := [ .move .nil (.imm false (.idx 2 0)) ]
+--   size _ := 0
+--   sound | (_, _) => by simp
 
-instance [Complexity.Computable Encoding.Model ↿Memory.getmp] [Complexity.Computable Encoding.Model Memory.getv]:
-    Trace.HasTrace ↿Memory.getvp where
-  program := [
-    .subroutine 0 0 ↿Memory.getmp,
-    .subroutine 0 0 Memory.getv
-  ]
-  size _ := 0
-  sound | (_, _) => by simp
+-- instance [Complexity.Computable Encoding.Model ↿Memory.getmp] [Complexity.Computable Encoding.Model Memory.getv]:
+--     Trace.HasTrace ↿Memory.getvp where
+--   program := [
+--     .subroutine 0 0 ↿Memory.getmp,
+--     .subroutine 0 0 Memory.getv
+--   ]
+--   size _ := 0
+--   sound | (_, _) => by simp
 
-instance: Trace.HasTrace ↿Memory.getmp where
-  program := [
-    .ifv 2 [
-      .move 1 (.imm false (.idx 5 0)),
-      .move 2 6,
-      .recurse 0 0
-    ],
-    .move 0 1
-  ]
-  size | (_, as) => as.length
-  sound | (_, as) => by cases as <;> simp
+-- instance: Trace.HasTrace ↿Memory.getmp where
+--   program := [
+--     .ifv 2 [
+--       .move 1 (.imm false (.idx 5 0)),
+--       .move 2 6,
+--       .recurse 0 0
+--     ],
+--     .move 0 1
+--   ]
+--   size | (_, as) => as.length
+--   sound | (_, as) => by cases as <;> simp
 
 
-instance [Complexity.Computable Encoding.Model ↿Memory.getvp] [Complexity.Computable Encoding.Model ↿(@List.cons Bool)]:
-  Trace.HasTrace ↿Source.get where
-  program := [
-    .ifv 1 [
-      .move 6 2,
-      .move 5 4,
-      .copy 4 6,
-      .recurse 2 2,
-      .ifv 3 [
-        .copy 8 4,
-        .setv 3 false,
-        .recurse 3 3,
-        .swap 3 4,
-        .setv 1 false,
-        .subroutine 1 1 ↿Memory.getvp,
-        .subroutine 0 0 ↿(@List.cons Bool)
-      ],
-      .move 1 7,
-      .subroutine 0 0 ↿(@List.cons Bool)
-    ],
-    .setm 0 0
-  ]
-  size | (s, _) => s.size
-  sound | (s, _) => by cases s <;> simp
+-- instance [Complexity.Computable Encoding.Model ↿Memory.getvp] [Complexity.Computable Encoding.Model ↿(@List.cons Bool)]:
+--   Trace.HasTrace ↿Source.get where
+--   program := [
+--     .ifv 1 [
+--       .move 6 2,
+--       .move 5 4,
+--       .copy 4 6,
+--       .recurse 2 2,
+--       .ifv 3 [
+--         .copy 8 4,
+--         .setv 3 false,
+--         .recurse 3 3,
+--         .swap 3 4,
+--         .setv 1 false,
+--         .subroutine 1 1 ↿Memory.getvp,
+--         .subroutine 0 0 ↿(@List.cons Bool)
+--       ],
+--       .move 1 7,
+--       .subroutine 0 0 ↿(@List.cons Bool)
+--     ],
+--     .setm 0 0
+--   ]
+--   size | (s, _) => s.size
+--   sound | (s, _) => by cases s <;> simp
 end HMem.Complexity
